impl_serialize_map_group_choice, zero_or_one, concat

src/cddl/pulse/CDDL.Pulse.Serialize.MapGroup.fst
@@ -85,3 +85,197 @@ let impl_serialize_map_group_ext'
 : impl_serialize_map_group #(Ghost.reveal t) #(Ghost.reveal fp') #tgt #inj (mg_spec_ext ps fp' ps.mg_size ps.mg_serializable) #impl_tgt r
 = impl_serialize_map_group_ext i _ ()
 
+inline_for_extraction noextract [@@noextract_to "krml"]
+fn impl_serialize_map_group_choice
+    (#[@@@erasable]t1: Ghost.erased det_map_group)
+    (#[@@@erasable]tgt1: Type0)
+    (#[@@@erasable] fp1: Ghost.erased typ)
+    (#[@@@erasable] inj1: Ghost.erased bool)
+    (#[@@@erasable]ps1: Ghost.erased (mg_spec t1 fp1 tgt1 inj1))
+    (#impl_tgt1: Type0)
+    (#[@@@erasable]r1: rel impl_tgt1 tgt1)
+    (i1: impl_serialize_map_group ps1 r1)
+    (#[@@@erasable]t2: Ghost.erased det_map_group)
+    (#[@@@erasable]tgt2: Type0)
+    (#[@@@erasable] fp2: Ghost.erased typ)
+    (#[@@@erasable] inj2: Ghost.erased bool)
+    (#[@@@erasable]ps2: Ghost.erased (mg_spec t2 fp2 tgt2 inj2))
+    (#impl_tgt2: Type0)
+    (#[@@@erasable]r2: rel impl_tgt2 tgt2)
+    (i2: impl_serialize_map_group ps2 r2)
+    (sq: squash (
+      map_group_footprint t1 fp1 /\
+      map_group_footprint t2 fp2 /\
+      map_group_choice_compatible t1 t2
+    ))
+: impl_serialize_map_group #_ #_ #_ #_ (mg_spec_choice ps1 ps2) #_ (rel_either r1 r2)
+=
+    (c: _)
+    (#v: _)
+    (out: _)
+    (out_count: _)
+    (out_size: _)
+    (l: _)
+{
+  rel_either_cases r1 r2 c v;
+  match c {
+    norewrite
+    Inl c1 -> {
+      Trade.rewrite_with_trade (rel_either r1 r2 c v) (r1 c1 (Inl?.v v));
+      let res = i1 c1 out out_count out_size l;
+      Trade.elim _ _;
+      res
+    }
+    norewrite
+    Inr c2 -> {
+      Trade.rewrite_with_trade (rel_either r1 r2 c v) (r2 c2 (Inr?.v v));
+      let res = i2 c2 out out_count out_size l;
+      Trade.elim _ _;
+      res
+    }
+  }
+}
+
+inline_for_extraction noextract [@@noextract_to "krml"]
+fn impl_serialize_map_group_zero_or_one
+    (#[@@@erasable]t1: Ghost.erased det_map_group)
+    (#[@@@erasable]tgt1: Type0)
+    (#[@@@erasable] fp1: Ghost.erased typ)
+    (#[@@@erasable] inj1: Ghost.erased bool)
+    (#[@@@erasable]ps1: Ghost.erased (mg_spec t1 fp1 tgt1 inj1))
+    (#impl_tgt1: Type0)
+    (#[@@@erasable]r1: rel impl_tgt1 tgt1)
+    (i1: impl_serialize_map_group ps1 r1)
+    (sq: squash (
+      map_group_footprint t1 fp1 /\
+      MapGroupFail? (apply_map_group_det t1 cbor_map_empty)
+    ))
+: impl_serialize_map_group #_ #_ #_ #_ (mg_spec_zero_or_one ps1) #_ (rel_option r1)
+=
+    (c: _)
+    (#v: _)
+    (out: _)
+    (out_count: _)
+    (out_size: _)
+    (l: _)
+{
+  rel_option_cases r1 c v;
+  match c {
+    norewrite
+    Some c1 -> {
+      Trade.rewrite_with_trade (rel_option r1 c v) (r1 c1 (Some?.v v));
+      let res = i1 c1 out out_count out_size l;
+      Trade.elim _ _;
+      res
+    }
+    norewrite
+    None -> {
+      true
+    }
+  }
+}
+
+let cbor_det_serialize_map_append_length_pat
+  (m1 m2: cbor_map)
+: Lemma
+  (requires (cbor_map_disjoint m1 m2))
+  (ensures (Seq.length (Cbor.cbor_det_serialize_map (cbor_map_union m1 m2)) == Seq.length (Cbor.cbor_det_serialize_map m1) + Seq.length (Cbor.cbor_det_serialize_map m2)))
+  [SMTPat (cbor_map_union m1 m2)]
+= Cbor.cbor_det_serialize_map_append_length m1 m2
+
+let mg_spec_concat_serializer_eq
+  (#source1: det_map_group)
+  (#source_fp1: typ)
+  (#target1: Type)
+  (#inj1: bool)
+  (p1: mg_spec source1 source_fp1 target1 inj1)
+  (#source2: det_map_group)
+  (#source_fp2: typ)
+  (#target2: Type)
+  (#inj2: bool)
+  (p2: mg_spec source2 source_fp2 target2 inj2 {
+    map_group_footprint source1 source_fp1 /\
+    map_group_footprint source2 source_fp2 /\
+    typ_disjoint source_fp1 source_fp2
+  })
+  (v: (target1 & target2))
+: Lemma
+  (ensures (
+    let mg = mg_spec_concat p1 p2 in
+    mg.mg_serializable v ==> (
+    p1.mg_serializable (fst v) /\
+    p2.mg_serializable (snd v) /\ (
+    let m1 = p1.mg_serializer (fst v) in
+    let m2 = p2.mg_serializer (snd v) in
+    cbor_map_disjoint m1 m2 /\
+    mg.mg_serializer v == cbor_map_union m1 m2
+  ))))
+= ()
+
+let cbor_map_union_assoc_pat (m1 m2 m3: cbor_map) : Lemma
+  (ensures (cbor_map_union (cbor_map_union m1 m2) m3 == cbor_map_union m1 (cbor_map_union m2 m3)))
+  [SMTPatOr [
+    [SMTPat (cbor_map_union (cbor_map_union m1 m2) m3)];
+    [SMTPat (cbor_map_union m1 (cbor_map_union m2 m3))]
+  ]]
+= cbor_map_union_assoc m1 m2 m3
+
+let cbor_map_length_disjoint_union_pat (m1 m2: cbor_map) : Lemma
+  (requires (cbor_map_disjoint m1 m2))
+  (ensures (
+    cbor_map_length (cbor_map_union m1 m2) == cbor_map_length m1 + cbor_map_length m2
+  ))
+  [SMTPat (cbor_map_union m1 m2)]
+= cbor_map_length_disjoint_union m1 m2
+
+#push-options "--z3rlimit 16"
+
+inline_for_extraction noextract [@@noextract_to "krml"]
+fn impl_serialize_map_group_concat
+    (#[@@@erasable]t1: Ghost.erased det_map_group)
+    (#[@@@erasable]tgt1: Type0)
+    (#[@@@erasable] fp1: Ghost.erased typ)
+    (#[@@@erasable] inj1: Ghost.erased bool)
+    (#[@@@erasable]ps1: Ghost.erased (mg_spec t1 fp1 tgt1 inj1))
+    (#impl_tgt1: Type0)
+    (#[@@@erasable]r1: rel impl_tgt1 tgt1)
+    (i1: impl_serialize_map_group ps1 r1)
+    (#[@@@erasable]t2: Ghost.erased det_map_group)
+    (#[@@@erasable]tgt2: Type0)
+    (#[@@@erasable] fp2: Ghost.erased typ)
+    (#[@@@erasable] inj2: Ghost.erased bool)
+    (#[@@@erasable]ps2: Ghost.erased (mg_spec t2 fp2 tgt2 inj2))
+    (#impl_tgt2: Type0)
+    (#[@@@erasable]r2: rel impl_tgt2 tgt2)
+    (i2: impl_serialize_map_group ps2 r2)
+    (sq: squash (
+      map_group_footprint t1 fp1 /\
+      map_group_footprint t2 fp2 /\
+      typ_disjoint fp1 fp2
+    ))
+: impl_serialize_map_group #_ #_ #_ #_ (mg_spec_concat ps1 ps2) #_ (rel_pair r1 r2)
+=
+    (c: _)
+    (#v: _)
+    (out: _)
+    (out_count: _)
+    (out_size: _)
+    (l: _)
+{
+  norewrite let (c1, c2) = c;
+  Trade.rewrite_with_trade (rel_pair r1 r2 c v) (r1 c1 (fst v) ** r2 c2 (snd v));
+  let res1 = i1 c1 out out_count out_size l;
+  S.pts_to_len out;
+  mg_spec_concat_serializer_eq ps1 ps2 v;
+  if (res1) {
+    let res2 = i2 c2 out out_count out_size (cbor_map_union l (ps1.mg_serializer (fst v)));
+    Trade.elim _ _;
+    S.pts_to_len out;
+    res2
+  } else {
+    Trade.elim _ _;
+    false
+  }
+}
+
+#pop-options
